f2effect: more on SfExtendPop
Ignore-this: 6c574121639eaa670eb530556b5f1855

darcs-hash:20131008075415-08f32-04866881f7e0042f84e983c7f5b66d94d4eb2ffa

done/Iron/Language/SystemF2Effect/Value/Merge.v
@@ -1,5 +1,6 @@
 
-Require Import Iron.Language.SystemF2Effect.Value.
+Require Import Iron.Language.SystemF2Effect.Value.Exp.
+Require Import Iron.Language.SystemF2Effect.Value.TyJudge.
 
 
 Fixpoint mergeT (p1 p2 : nat) (tt : ty)  : ty :=
@@ -14,26 +15,140 @@ Fixpoint mergeT (p1 p2 : nat) (tt : ty)  : ty :=
  | TCon2   tc2 t1 t2    => TCon2 tc2 (mergeT p1 p2 t1) (mergeT p1 p2 t2)
  | TCap (TyCapRegion p) => if beq_nat p p2 then TRgn p1 else tt
  end.
-    
+
 
 Fixpoint mergeV (p1 p2 : nat) (vv : val) : val :=
  match vv with
- | VVar  _       => vv
- | VLoc  _       => vv
- | VLam  t x     => VLam (mergeT p1 p2 t) (mergeX p1 p2 x)
- | VLAM  k x     => VLAM k (mergeX p1 p2 x)
- | VConst c      => vv
+ | VVar  _        => vv
+ | VLoc  _        => vv
+ | VLam  t x      => VLam     (mergeT p1 p2 t) (mergeX p1 p2 x)
+ | VLAM  k x      => VLAM k   (mergeX p1 p2 x)
+ | VConst c       => vv
  end
  with   mergeX (p1 p2 : nat) (xx : exp) : exp :=
  match xx with
- | XVal v        => XVal (mergeV p1 p2 v)
- | ...
+ |  XVal v         
+ => XVal     (mergeV p1 p2 v)
 
-  
+ |  XLet t x1 x2   
+ => XLet     (mergeT p1 p2 t)  (mergeX p1 p2 x1) (mergeX p1 p2 x2)
+
+ |  XApp v1 v2     
+ => XApp     (mergeV p1 p2 v1) (mergeV p1 p2 v2)
+
+ |  XAPP v1 t2     
+ => XAPP     (mergeV p1 p2 v1) (mergeT p1 p2 t2)
+
+ |  XOp1 op v      
+ => XOp1 op  (mergeV p1 p2 v)
+
+ |  XPrivate x     
+ => XPrivate (mergeX p1 p2 x)
+
+ |  XExtend  t x   
+ => XExtend  (mergeT p1 p2 t)  (mergeX p1 p2 x)
+
+ |  XAlloc t v     
+ => XAlloc   (mergeT p1 p2 t)  (mergeV p1 p2 v)
+
+ |  XRead  t v     
+ => XRead    (mergeT p1 p2 t)  (mergeV p1 p2 v)
+
+ |  XWrite t v1 v2 
+ => XWrite   (mergeT p1 p2 t)  (mergeV p1 p2 v1) (mergeV p1 p2 v2)
+ end.
 
 
-Lemma typev_merge 
- : forall 
- ,  TYPEV ke te se sp v (substTT 0 (TRgn p2) t)
- -> TYPEV ke (mergeTE p1 p2 te) (mergeSE p1 p2 se) sp 
-             (mergeV  p1 p2 v)  (substTT 0 (TRgn p1) t).
+Definition mergeTE p1 p2 te := map (mergeT p1 p2) te.
+Hint Unfold mergeTE.
+
+
+Definition mergeSE p1 p2 se := map (mergeT p1 p2) se.
+Hint Unfold mergeSE.
+
+
+(********************************************************************)
+Lemma typex_merge 
+ : forall ix ke te se sp x t e p1 p2
+ ,  TYPEX ke te se sp 
+          x                 (substTT ix (TRgn p2) t) (substTT ix (TRgn p2) e)
+ -> TYPEX ke                (mergeTE p1 p2 te)       (mergeSE p1 p2 se) sp 
+          (mergeX  p1 p2 x) (substTT ix (TRgn p1) t) (substTT ix (TRgn p1) e).
+Proof.
+ intros. gen ke te se sp t e.
+ induction x using exp_mutind with
+  (PV := fun v => forall ke te se sp t
+      ,  get ix ke = Some KRegion
+      -> TYPEV ke te se sp v     (substTT ix (TRgn p2) t)  
+      -> TYPEV ke                (mergeTE p1 p2 te) (mergeSE p1 p2 se) sp
+               (mergeV  p1 p2 v) (substTT ix (TRgn p1) t));
+  intros.
+
+ - Case "VVar".
+   admit.
+
+ - Case "VLoc".
+   admit.
+
+ - Case "VLam".
+   inverts H0.
+   destruct t0;       try (snorm; congruence).
+   inverts H7.
+   destruct t0_1;     try (snorm; congruence).
+   simpl in H1. inverts H1.
+   destruct t0_1_1;   try (snorm; congruence).
+   simpl in H2. inverts H2.
+   destruct t0_1_1_1; try (snorm; congruence).
+   simpl in H1. inverts H1.
+   simpl.
+   rrwrite ( mergeT p1 p2 (substTT ix (TRgn p2) t0_1_1_2)
+           = substTT ix (TRgn p1) t0_1_1_2) by admit.
+   eapply TvLam. 
+   + admit.                                  (* fix kind  of TRgn p1 *)
+   + eapply IHx in H9; auto.
+     simpl in H9.
+     admit.
+
+ - Case "VLAM".
+   snorm.
+   admit.
+
+ - Case "VConst".
+   snorm. 
+   eapply TvConst.
+   destruct c; inverts H0; snorm.
+   + destruct t; snorm; nope.
+   + destruct t; snorm; nope.
+   + destruct t; snorm; nope.
+
+ - Case "VVal".
+   admit.
+
+ - Case "XLet".
+   admit.
+
+ - Case "XApp".
+   admit.
+
+ - Case "XAPP".
+   admit.
+
+ - Case "XOp1".
+   admit.
+
+ - Case "XPrivate".
+   admit.
+
+ - Case "XExtend".
+   admit.
+
+ - Case "XAlloc".
+   admit.
+
+ - Case "XRead".
+   admit.
+
+ - Case "XWrite".
+   admit.
+Qed.
+
